Remove Refine Instance Mode option

test-suite/success/Typeclasses.v
@@ -198,9 +198,7 @@ Module UniqueInstances.
       for it. *)
   Set Typeclasses Unique Instances.
   Class Eq (A : Type) : Set.
-    Set Refine Instance Mode.
-    Instance eqa : Eq nat := _. constructor. Qed.
-    Unset Refine Instance Mode.
+    Instance eqa : Eq nat. Qed.
     Instance eqb : Eq nat := {}.
     Class Foo (A : Type) (e : Eq A) : Set.
     Instance fooa : Foo _ eqa := {}.
